theories/overlay/base.v
@@ -1,0 +1,63 @@
+From iris.algebra Require Import base.
+From iris.program_logic Require Import language ectx_language ectxi_language.
+From stdpp Require Import gmap fin_maps list finite.
+From cap_machine Require Export addr_reg machine_base machine_parameters.
+
+Inductive Cap: Type :=
+| Regular: machine_base.Cap -> Cap (* Regular capabilities *)
+| Stk: nat -> Perm -> Addr -> Addr -> Addr -> Cap (* Stack derived capabilities *)
+| Ret: nat -> Addr -> Addr -> Addr -> Cap. (* Return capabilities *)
+
+Instance cap_eq_dec : EqDecision Cap.
+Proof. solve_decision. Defined.
+Instance word_eq_dec : EqDecision Word.
+Proof. solve_decision. Defined.
+
+Definition Word := (Z + Cap)%type.
+
+Notation Reg := (gmap RegName Word).
+Notation Mem := (gmap Addr Word).
+
+Definition RegLocate (reg : Reg) (r : RegName) :=
+  match (reg !! r) with
+  | Some w => w
+  | None => inl 0%Z
+  end.
+
+Definition MemLocate (mem : Mem) (a : Addr) :=
+  match (mem !! a) with
+  | Some w => w
+  | None => inl 0%Z
+  end.
+
+Notation "mem !m! a" := (MemLocate mem a) (at level 20).
+Notation "reg !r! r" := (RegLocate reg r) (at level 20).
+
+Definition Stackframe := (Reg * Mem)%type.
+
+Definition ExecConf := (Reg * Mem * Mem * list Stackframe)%type.
+
+Definition reg (ϕ: ExecConf) :=
+  match ϕ with
+  | (r, _, _, _) => r
+  end.
+
+Definition mem (ϕ: ExecConf) :=
+  match ϕ with
+  | (_, m, _, _) => m
+  end.
+
+Definition stk (ϕ: ExecConf) :=
+  match ϕ with
+  | (_, _, stk, _) => stk
+  end.
+
+Definition callstack (ϕ: ExecConf) :=
+  match ϕ with
+  | (_, _, _, cs) => cs
+  end.
+
+Lemma ExecConfDestruct:
+  forall ϕ,
+    ϕ = (reg ϕ, mem ϕ, stk ϕ, callstack ϕ).
+Proof. repeat destruct ϕ as (ϕ & ?). reflexivity. Qed.
