theories/overlay/call.v
@@ -1,0 +1,50 @@
+From iris.algebra Require Import base.
+From iris.program_logic Require Import language ectx_language ectxi_language.
+From stdpp Require Import gmap fin_maps list finite.
+From cap_machine Require Export addr_reg machine_base machine_parameters.
+From cap_machine.overlay Require Import base.
+
+(* Call r rargs implements a calling convention with arguments passed on the stack
+   Assuming that r0, r1 ∉ {r, rargs}, and r_stk contains a stack capability, it will
+   - save *all* registers on the stack except PC and r_stk
+   - prepare the return capability
+   - prepare the stack capability in r_stk for a new frame
+   - push the return capability
+   - push all arguments
+   - clear all registers except PC, r and r_stk
+   - jmp r *)
+
+Section call.
+
+  Context `{MachineParameters}.
+  Parameter r_stk: RegName.
+
+  (* Clearing a list of registers *)
+  Definition rclear_instrs (r : list RegName): list Word := map (λ r_i, inl (encodeInstr (Mov r_i (inl 0%Z)))) r.
+
+  (* Push instruction *)
+  Definition push_instrs ρs: list Word := map (fun ρ => inl (encodeInstr (StoreU r_stk (inl 0%Z) ρ))) ρs.
+
+  (* Pop instruction *)
+  Definition pop_instrs r: list Word := [inl (encodeInstr (LoadU r r_stk (inl (-1)%Z))); inl (encodeInstr (Lea r_stk (inl (-1)%Z)))].
+
+  (* Push all registers except r_stk and PC *)
+  Definition push_env_instrs: list Word :=
+    push_instrs (map (fun r => inr r) (list_difference all_registers [PC; r_stk])).
+
+  (* Pop all registers except r_stk and PC, must be reverse order from push *)
+  Definition pop_env_instrs: list Word :=
+    foldl (fun b r => (pop_instrs r) ++ b) [] (list_difference all_registers [PC; r_stk]).
+
+  (* Code for call macro *)
+  Definition call_instrs r rargs: list Word :=
+    push_env_instrs
+    ++ [(* TODO: prepare return capability *)]
+    ++ [(* TODO: prepare stack capability *)]
+    ++ [(* TODO: push return capability *)]
+    ++ push_instrs (map (fun r => inr r) rargs)
+    ++ rclear_instrs (list_difference all_registers [PC; r; r_stk])
+    ++ [inl (encodeInstr (Jmp r))]
+    ++ pop_env_instrs.
+
+End call.
